\item Hallar los lÃ­mites de las sucesiones dadas por:
\begin{multicols}{2}
    \begin{enumerate}
    \item $\D a_n = \Big( \frac{2n^2+3n-1}{3n^2-6n+1} \Big)^{2n}$
    \item $\D a_n = \Big( \frac{3n+4}{2n+5} \Big)^{\sqrt{n+1}-\sqrt{n}}$
    \item $\D a_n = \Big( \frac{3n+4}{3n-5} \Big)^{n}$
    \item $\D a_n = \Big( \frac{3n+4}{3n-5} \Big)^{n^2}$
    \item $\D a_n = \Big( \frac{3n+4}{3n-5} \Big)^{\sqrt{n}}$
    \item $\D a_n = \frac{\ln n}n$
    \end{enumerate}
\end{multicols}

\item Probar $\lim a_n = +\infty$ y $\lim b_n = b > 0$, entonces $\lim a_n^{b_n} = +\infty$.

\item Probar que si $\lim a_n = a > 1$ y $\lim b_n = +\infty$,
entonces $\lim a_n^{b_n} = +\infty$.
